Changes from some time ago: tried to solve an exercise about scheduling, but failed. Started a file with binary heaps and implemented makeHeap.

Sorting/InsertionSort.v
@@ -44,3 +44,49 @@ Proof.
   induction l as [| h t]; simpl; auto.
     apply perm_trans with (h :: insertionSort A t); auto. apply perm_ins.
 Defined.
+
+(** Better insertion sort. *)
+
+Fixpoint ins'
+  {A : Type} (cmp : A -> A -> bool) (x : A) (l : list A) : list A :=
+match l with
+    | [] => [x]
+    | h :: t => if cmp x h then x :: h :: t else h :: (ins' cmp x t)
+end.
+
+Definition insertionSort'
+  {A : Type} (cmp : A -> A -> bool) (l : list A) : list A :=
+    fold_right (ins' cmp) [] l.
+
+Coercion leqb : LinDec >-> Funclass.
+
+Lemma perm_ins' :
+  forall (A : LinDec) (x : A) (l : list A),
+    perm A (x :: l) (ins' A x l).
+Proof.
+  unfold perm. induction l; cbn; intros.
+    reflexivity.
+    unfold ins'; destruct (leqb x a); fold (@ins' A).
+      reflexivity.
+      dec; rewrite <- IHl; cbn; dec.
+Qed.
+
+Lemma sorted_ins' :
+  forall (A : LinDec) (x : A) (l : list A),
+    sorted A l -> sorted A (ins' A x l).
+Proof.
+  induction l as [| h t]; cbn; intros.
+    constructor.
+    dec. induction t as [| h' t']; cbn in *; dec.
+Qed.
+
+Instance Sort_insertionSort' (A : LinDec) : Sort A :=
+{
+    sort := insertionSort' A
+}.
+Proof.
+  induction l as [| h t]; cbn; auto.
+    apply sorted_ins'. assumption.
+  induction l as [| h t]; simpl; auto.
+    apply perm_trans with (h :: insertionSort' A t), perm_ins'; auto.
+Defined.
