DS/Heap.v
@@ -1,0 +1,237 @@
+Add Rec LoadPath "/home/zeimer/Code/Coq".
+
+Require Import BTree.
+Require Export LinDec.
+Require Import Sorting.Sort.
+
+Definition minmax {A : LinDec} (x y : A) : A * A :=
+  if x <=? y then (x, y) else (y, x).
+
+Definition min {A : LinDec} (x y : A) : A :=
+  if x <=? y then x else y.
+
+Definition max {A : LinDec} (x y : A) : A :=
+  if y <=? x then x else y.
+
+Function sendDown {A : LinDec} (x : A) (t : BTree A) : A * BTree A :=
+match t with
+    | empty => (x, empty)
+    | node v l r =>
+        let
+          '(m, M) := minmax x v
+        in
+          match l, r with
+              | empty, empty => (m, (node M l r))
+              | empty, _ =>
+                  let '(m', r') := sendDown M r in
+                    (min m m', node (max m m') l r')
+              | _, empty =>
+                  let '(m', l') := sendDown M l in
+                    (min m m', node (max m m') l' r)
+              | node vl _ _, node vr _ _ =>
+                  if vl <=? vr
+                  then
+                    let '(m', l') := sendDown M l in
+                      (min m m', node (max m m') l' r)
+                  else
+                    let '(m', r') := sendDown M r in
+                      (min m m', node (max m m') l r')
+          end
+end.
+
+Compute @sendDown natle
+  2 (node 4 (node 10 empty empty) (node 8 empty empty)).
+
+Lemma sendDown_elem :
+  forall (A : LinDec) (x m : A) (t t' : BTree A),
+    sendDown x t = (m, t') ->
+      x = m \/ elem x t'.
+Proof.
+  intros. functional induction @sendDown A x t; inv H; dec;
+  repeat match goal with
+      | H : match ?x with _ => _ end |- _ => destruct x
+      | H : False |- _ => contradiction
+      | IH : forall _ _, _ -> _, H : sendDown _ _ = _ |- _ =>
+          destruct (IH _ _ H); clear IH; subst
+  end;
+  unfold min, max, minmax in *; dec; inv e0.
+Qed.
+
+Lemma sendDown_elem' :
+  forall (A : LinDec) (x m y : A) (t t' : BTree A),
+    sendDown x t = (m, t') -> elem y t -> y = m \/ elem y t'.
+Proof.
+Admitted.
+
+Lemma sendDown_elem'' :
+  forall (A : LinDec) (x m y : A) (t t' : BTree A),
+    sendDown x t = (m, t') -> elem y t ->
+      (x = m /\ t = t') \/
+      (y = m \/ elem x t').
+Proof.
+Admitted.
+
+(*Lemma isHeap_sendDown :
+  forall (A : LinDec) (x m : A) (t t' : BTree A),
+    isHeap t -> sendDown x t = (m, t') ->
+      isHeap t' /\ forall a : A, elem a t' -> m ≤ a.
+Proof.
+  intros. functional induction @sendDown A x t; inv H0.
+    split; [constructor | inv 1].
+    split.
+      repeat constructor; inv 1.
+      inv 1; try inv H2. unfold minmax in e0; dec. inv e0.
+    destruct _x.
+      contradiction.
+      inv H. destruct (IHp _ _ H6 e3); clear IHp y. split.
+        repeat constructor.
+          inv 1.
+          intros. unfold max, minmax in *. dec; inv e0.
+Admitted.
+*)
+
+Function makeHeap {A : LinDec} (t : BTree A) : BTree A :=
+match t with
+    | empty => empty
+    | node v l r =>
+        match makeHeap l, makeHeap r with
+            | empty, empty => node v empty empty
+            | empty, r' =>
+                let '(m, r'') := sendDown v r' in node m empty r''
+            | l', empty =>
+                let '(m, l'') := sendDown v l' in node m l'' empty
+            | node vl _ _ as l', node vr _ _ as r' =>
+                if vl <=? vr
+                then let '(m, l'') := sendDown v l' in node m l'' r'
+                else let '(m, r'') := sendDown v r' in node m l' r''
+        end
+end.
+
+Ltac dec' := cbn;
+repeat match goal with
+    | |- context [?x =? ?y] =>
+        try destruct (LinDec_eqb_spec natle x y);
+        try destruct (LinDec_eqb_spec _ x y); subst; intros
+    | |- context [?x <=? ?y] =>
+        try destruct (@leqb_spec natle x y);
+        try destruct (leqb_spec x y); intros
+    | H : context [?x =? ?y] |- _ =>
+        try destruct (LinDec_eqb_spec natle x y);
+        try destruct (LinDec_eqb_spec _ x y); subst; intros
+    | H : context [?x <=? ?y] |- _ =>
+        try destruct (@leqb_spec natle x y);
+        try destruct (leqb_spec x y); intros
+end; cbn;
+repeat match goal with
+    | H : ?x <> ?x |- _ => contradiction H; reflexivity
+    | H : True |- _ => clear H
+    | H : ?x = ?x |- _ => clear H
+end; try congruence.
+
+Inductive ih {A : LinDec} : BTree A -> Prop :=
+    | ih_empty : ih empty
+    | ih_singl : forall v : A, ih (node v empty empty)
+    | ih_l :
+        forall (v x : A) (l r : BTree A),
+          v ≤ x -> ih (node x l r) -> ih (node v (node x l r) empty)
+    | ih_r :
+        forall (v x : A) (l r : BTree A),
+          v ≤ x -> ih (node x l r) -> ih (node v empty (node x l r))
+    | ih_lr :
+        forall (v lv rv : A) (ll lr rl rr : BTree A),
+          v ≤ lv -> ih (node lv ll lr) ->
+          v ≤ rv -> ih (node rv rl rr) ->
+            ih (node v (node lv ll lr) (node rv rl rr)).
+
+Lemma minmax_leq :
+  forall (A : LinDec) (x y m M : A),
+    minmax x y = (m, M) -> m ≤ M.
+Proof.
+  unfold minmax. intros. dec. inv H.
+Qed.
+
+Lemma leq_min_max :
+  forall (A : LinDec) (x y : A),
+    min x y ≤ max x y.
+Proof.
+  unfold min, max. intros. dec.
+Qed.
+
+Lemma sendDown_ih :
+  forall (A : LinDec) (x m : A) (t t' : BTree A),
+    sendDown x t = (m, t') ->
+      t = empty /\ t' = empty \/
+      exists (v : A) (l r : BTree A),
+        t' = node v l r /\ ih t' /\ m ≤ v.
+Proof.
+  intros. functional induction @sendDown A x t; inv H; right.
+    exists M, empty, empty. repeat split.
+      constructor.
+      eapply minmax_leq. eauto.
+    do 3 eexists. repeat split.
+      2: apply leq_min_max.
+      decompose [and or ex] (IHp _ _ e3); clear IHp; subst.
+        contradiction.
+        constructor.
+Admitted.
+(*
+        contradiction.
+        constructor.
+          apply minmax_leq in e0. unfold max; dec. inv e0.
+      eauto.
+      apply leq_min_max.
+    do 3 eexists. split.
+      eauto.
+      apply leq_min_max.
+    do 3 eexists. split.
+      eauto.
+      apply leq_min_max.
+    do 3 eexists. split.
+      eauto.
+      apply leq_min_max.
+Qed.*)
+
+Lemma ih_sendDown_arg :
+  forall (A : LinDec) (x m : A) (t t' : BTree A),
+    sendDown x t = (m, t') -> ih t ->
+      forall a : A, elem a t -> m ≤ a.
+Proof.
+  intros. functional induction @sendDown A x t.
+Abort.
+
+Lemma ih_sendDown_res :
+  forall (A : LinDec) (x m : A) (t t' : BTree A),
+    sendDown x t = (m, t') -> ih t ->
+      forall a : A, elem a t' -> m ≤ a.
+Proof.
+Admitted.
+
+Lemma makeHeap_ih :
+  forall (A : LinDec) (t : BTree A),
+    ih (makeHeap t).
+Proof.
+  intros. functional induction @makeHeap A t;
+  repeat match goal with
+      | H : match ?x with _ => _ end |- _ => destruct x eqn: Hx
+      | H : False |- _ => contradiction
+      | H : True |- _ => clear H
+      | H : elem _ empty |- _ => inv H
+      | H : makeHeap _ = _ |- _ => rewrite ?H in *; clear H
+      | H : ih empty |- _ => clear H
+  end;
+  try match goal with
+      | H : sendDown _ _ = _ |- _ =>
+          let H' := fresh "H" in 
+          assert (H' := sendDown_ih _ _ _ _ _ H);
+          decompose [and or ex] H'; clear H'; subst
+  end;
+  constructor; try assumption; try congruence.
+    eapply leq_trans with vl.
+      eapply ih_sendDown_arg; eauto.
+      dec'.
+    eapply leq_trans with vr.
+      eapply ih_sendDown_arg; eauto.
+      dec.
+Qed.
+
+Print Assumptions makeHeap_ih.
